lawyer/nonblocking/examples/queue/simple_queue_spec.v
@@ -8,11 +8,11 @@ From lawyer.obligations Require Import obligations_model obligations_resources o
 From lawyer Require Import sub_action_em program_logic.
 From iris.algebra Require Import auth gmap gset excl excl_auth csum mono_nat.
 From iris.base_logic.lib Require Import invariants.
-From lawyer.nonblocking.examples.queue Require Import simple_queue_utils simple_queue init_queue.
+From lawyer.nonblocking.examples.queue Require Import simple_queue_utils simple_queue init_queue wrappers_lib.
+From lawyer.nonblocking.tokens Require Import om_wfree_inst_tokens tokens_ra.
 From lawyer.nonblocking.examples.queue.dequeuer Require Import dequeuer_thread. 
 From lawyer.nonblocking.examples.queue.enqueuer Require Import enqueuer_thread. 
 From heap_lang Require Import heap_lang_defs lang notation.
-From lawyer.nonblocking.tokens Require Import om_wfree_inst_tokens tokens_ra. 
 
 Close Scope Z.
 
@@ -22,60 +22,64 @@ Section QueueSpec.
 
   Definition queue_ms: gmultiset val := {[+ enqueuer_thread SQ; dequeuer_thread SQ +]}.
 
-  (* TODO: move all of this *)
-  (**************************)
-  Definition max_exact_Σ: gFunctors := #[ GFunctor (prodUR (excl_authUR nat) mono_natUR)].
-  Global Instance max_exact_sub: forall Σ, subG max_exact_Σ Σ -> MaxExactPreG Σ.
-  Proof using. solve_inG. Qed. 
-  
-  Definition hist_queue_Σ: gFunctors := #[ GFunctor (authUR (gmapUR nat (agreeR HistNode)))].
-  Global Instance hist_queue_sub: forall Σ, subG hist_queue_Σ Σ -> HistQueuePreG Σ.
-  Proof using. solve_inG. Qed. 
-
-
-  Definition read_hist_Σ: gFunctors := #[ GFunctor (authUR (gmapUR nat (prodR
-                                    (optionR $ prodR (agreeR nat) max_natUR)
-                                    (optionR read_state_cmra)
-                                    )))].
-  Global Instance read_hist_sub: forall Σ, subG read_hist_Σ Σ -> ReadHistPreG Σ.
-  Proof using. solve_inG. Qed. 
-
-  (* q_pre_dangle_rop ::  inG Σ (excl_authUR (option nat)); *)
-  (* q_pre_tok :: inG Σ (exclR unitO); *)
-
   (* Instance queue_tokens_pre: SimpleQueueTokensPre mt_Σ. *)
-  Instance queue_tokens_pre: forall Σ, subG mt_Σ Σ -> SimpleQueueTokensPre Σ.
-  Proof using SQ.
-    constructor.
-    iMod (mt_init queue_ms) as "(%MT & TOKS)". iModIntro.
-    iExists (SQT _ _ _ _ _ _ _).
-    rewrite /queue_ms. rewrite methods_toks_split.
-    rewrite bi.sep_comm. iApply "TOKS".
-    Unshelve.
-    3, 4: by apply _.
-    1, 2: rewrite bi.wand_curry; rewrite -methods_toks_split;
-      iIntros "X"; iDestruct (methods_toks_sub with "X") as %V;
-      multiset_solver.
-  Qed. 
+  Program Instance mt_sqt Σ (MT: MethodToken queue_ms Σ): SimpleQueueTokens Σ := 
+    {| dequeue_token := method_tok (dequeuer_thread SQ);
+       read_head_token := method_tok (enqueuer_thread SQ); |}.
+  Solve Obligations with 
+    intros; rewrite bi.wand_curry; rewrite -methods_toks_split;
+    iIntros "X"; iDestruct (methods_toks_sub with "X") as %V;
+    multiset_solver.
+  Fail Next Obligation. 
 
-  Definition queue_Σ: gFunctors := #[
-    max_exact_Σ;
-    GFunctor (exclR unitO);
-    hist_queue_Σ;
-    read_hist_Σ; 
-    GFunctor (excl_authUR (option nat));
-    mt_Σ
-  ].
+  Existing Instance mt_sqt. 
 
-  Global Instance queue_sub: forall Σ, subG queue_Σ Σ -> QueuePreG Σ.
-  Proof using SQ. solve_inG. Qed. 
-
-  (**************************)
-
+  Lemma init_queue_inv {Σ} {hGS: heap1GS Σ} {iGS: invGS_gen HasNoLc Σ}
+    {MTPre: MethodTokenPre Σ} {QPre: QueuePreG Σ}:
+      ∀ c, is_init_queue_cfg SQ ph pfl #0 c → 
+            hl_phys_init_resource c ={⊤}=∗ 
+            ∃ (MT: MethodToken queue_ms Σ) (_: QueueG Σ),
+              queue_inv val_is_int ∗ methods_toks queue_ms (H := MT).
+  Proof using.
+    iIntros (c INIT) "HEAP".
+    iMod (mt_init queue_ms) as "(%MT & TOKS)". 
+    iDestruct (obtain_queue_init_resource with "[$]") as "QI"; eauto.
+    iMod (queue_init val_is_int with "QI []") as "(%QQ & QI)".
+    { set_solver. }
+    by iFrame.
+  Qed.
+ 
   Program Definition SimpleQueue_WaitFreeToken: WaitFreeSpecToken queue_ms := {|
     wfst_is_init_st := is_init_queue_cfg SQ ph pfl #0;
     wfst_preG := QueuePreG;
     wfst_G := QueueG;
     wfst_Σ := queue_Σ;
-    wfst_mod_inv := 
+    wfst_subG := queue_sub;
+    wfst_mod_inv _ _ _ _ _ := queue_inv val_is_int;
+    wfst_init_mod _ _ _ _ _ := init_queue_inv;
+    wfst_F := max et_fuel dt_fuel;
   |}.
+  Next Obligation.
+    iIntros "* #INV".
+    iApply big_sepS_forall. iIntros (m DOM).
+    rewrite /method_spec_token. iIntros (???? Φ) "!> (CPS & PH & TOK) POST".
+    apply gmultiset_elem_of_dom in DOM. rewrite /queue_ms in DOM.
+    rewrite gmultiset_elem_of_disj_union !gmultiset_elem_of_singleton in DOM.
+    destruct DOM as [-> | ->].
+    - split_cps "CPS" et_fuel.
+      replace CannotFork with CanFork by admit.
+      iApply (enqueuer_thread_spec with "[-POST]").
+      { iFrame "#∗". }
+      iIntros "!> %v (PH & RH & %GV)".
+      iApply "POST". iFrame.
+    - split_cps "CPS" et_fuel.
+      replace CannotFork with CanFork by admit.
+      iApply (dequeuer_thread_spec with "[-POST]").
+      { iFrame "#∗". }
+      iIntros "!> %v (PH & RH & %GV)".
+      iApply "POST". iFrame.
+  Admitted.
+  Final Obligation. 
+  Admitted. 
+
+End QueueSpec. 
