lawyer/nonblocking/examples/queue/wrappers_lib.v
@@ -1,0 +1,4 @@
+From heap_lang Require Import lang notation.
+
+
+Definition val_is_int {Σ: gFunctors} (v: val): iProp Σ := ⌜ ∃ (n: Z), v = #n ⌝.
